src/IOArray.thy
@@ -2,23 +2,26 @@ theory IOArray
   imports IO
 begin
 
-datatype 'a io_array = IOArray "'a ref" nat
+datatype 'a io_array = IOArray "'a array" nat
+
+primrec get_array_addr :: "'a::heap io_array \<Rightarrow> addr" where
+  "get_array_addr (IOArray a _) = addr_of_array a"
 
 primrec get_size :: "'a io_array \<Rightarrow> nat" where
   "get_size (IOArray _ s) = s"
 
 term "allocate"
 
-fun new_array :: "nat \<Rightarrow> 'a::heap io_array io" where
+definition new_array :: "nat \<Rightarrow> 'a::heap io_array io" where
   "new_array s = alloc s \<bind> (\<lambda>r. return (IOArray r s))"
 
-fun read_array :: "'a io_array \<Rightarrow> nat \<Rightarrow> 'a::heap io" where
-  "read_array (IOArray arr _) i = lookup (Ref (addr_of_ref arr + i))"
+definition read_array :: "'a io_array \<Rightarrow> nat \<Rightarrow> 'a::heap io" where
+  "read_array arr i = lookup (Ref (get_array_addr arr + i))"
 
-fun write_array :: "'a io_array \<Rightarrow> nat \<Rightarrow> 'a::heap \<Rightarrow> unit io" where
-  "write_array (IOArray arr _) i val = update (Ref (addr_of_ref arr + i)) val"
+definition write_array :: "'a io_array \<Rightarrow> nat \<Rightarrow> 'a::heap \<Rightarrow> unit io" where
+  "write_array arr i val = update (Ref (get_array_addr arr + i)) val"
 
-fun swap_array :: "'a::heap io_array \<Rightarrow> nat \<Rightarrow> nat \<Rightarrow> unit io" where
+definition swap_array :: "'a::heap io_array \<Rightarrow> nat \<Rightarrow> nat \<Rightarrow> unit io" where
   "swap_array arr i j = do {
     valI \<leftarrow> read_array arr i;
     valJ \<leftarrow> read_array arr j;
@@ -27,15 +30,27 @@ fun swap_array :: "'a::heap io_array \<Rightarrow> nat \<Rightarrow> nat \<Right
     return ()
   }"
 
+lemma execute_write_array: "execute_io (write_array arr n v) h = Some ((), set_heap (Ref (get_array_addr arr + n)) v h)"
+  by (simp add: execute_io_def update_def heap_def write_array_def)
+
+lemma write_write_array: "execute_io (write_array arr n x \<bind> (\<lambda>_. write_array arr n y)) h = execute_io (write_array arr n y) h"
+  by (simp add: execute_write_array)
+
 (* IO Operations *)
-fun write_list_as_array :: "'a::heap list \<Rightarrow> 'a io_array io" where
-  "write_list_as_array xs = (do {
+fun new_array_from_list :: "'a::heap list \<Rightarrow> 'a io_array io" where
+  "new_array_from_list xs = (do {
     arr \<leftarrow> new_array (size xs);
     forMu (enumerate 0 xs) (\<lambda>(i,x). write_array arr i x);
     return arr
   })"
 
-fun read_list_from_array :: "'a::heap io_array \<Rightarrow> 'a list io" where
-  "read_list_from_array (IOArray arr n) = mapM (\<lambda>i. read_array (IOArray arr n) i) (map nat [0..int n])"
+fun read_array_as_list :: "'a::heap io_array \<Rightarrow> 'a list io" where
+  "read_array_as_list (IOArray arr n) = mapM (\<lambda>i. read_array (IOArray arr n) i) (map nat [0..int n])"
+
+lemma effectE_new_array_from_list_index:
+  assumes "effect_io (new_array_from_list xs) h h' arr"
+  shows "get_array_addr arr = addr_of_array (fst (alloc_heap_array (size xs) h))" "h' = fold (\<lambda>(i,x). set_heap (Ref (get_array_addr arr + i)) x) (enumerate 0 xs) (snd (alloc_heap_array (size xs) h))"
+  using assms
+  sorry
 
 end
